start adding complete binary tree

Auto/Lib/BinTree.lean
@@ -5,6 +5,7 @@ import Auto.Lib.NatExtra
 import Auto.Lib.OptionExtra
 import Auto.Lib.Containers
 import Auto.Lib.Pos
+import Auto.Lib.Bin
 -- Make sure that `Lean.toExpr Nat` is overriden
 import Auto.Lib.ToExprExtra
 
@@ -15,32 +16,6 @@ import Auto.Lib.ToExprExtra
 -/
 
 namespace Auto
-
-open ToExprExtra
-
-namespace Bin
-
-private theorem wfAux (n : Nat) : (n + 2).div 2 < n + 2 := by
-  apply Nat.div_lt_self
-  case hLtN => apply Nat.succ_le_succ; apply Nat.zero_le
-  case hLtK => apply Nat.le_refl
-
-def inductionOn.{u}
-  {motive : Nat → Sort u} (x : Nat)
-  (ind : ∀ x, motive ((x + 2) / 2) → motive (x + 2))
-  (base₀ : motive 0) (base₁ : motive 1) : motive x :=
-  match x with
-  | 0 => base₀
-  | 1 => base₁
-  | x' + 2 => ind x' (inductionOn ((x' + 2) / 2) ind base₀ base₁)
-
-@[irreducible] def induction.{u}
-  {motive : Nat → Sort u}
-  (ind : ∀ x, motive ((x + 2) / 2) → motive (x + 2))
-  (base₀ : motive 0) (base₁ : motive 1) : ∀ x, motive x :=
-  fun x => inductionOn x ind base₀ base₁
-
-end Bin
 
 inductive BinTree (α : Type u) where
   | leaf : BinTree α
